interface coq-caml

coq/api.v
@@ -1,60 +1,192 @@
+Add LoadPath "$HOME/COQ/FO-LTL" as Top.
+
 Require Import List.
 Require Import String.
 
+Require Import Top.utils.
+
 Definition mlSort := string.
 
-Record mlRelation := {
-  mlRelName : string;
-  mlRelProfile : list mlSort;
-  mlRelArity := List.length mlRelProfile;
-}.
-
-Record mlConstant := {
-  mlCstName : string;
-  mlCstSort : mlSort;
-}.
-
-Record mlVar := {
-  mlVarId : nat;
-  mlVarName: string;
-  mlVarSort : mlSort;
-}.
-
 Record mlPath := {
-  mlTC : mlRelation;
-  mlBase : mlRelation;
+  mlTC : string;
+  mlBase : string;
 }.
+
+Inductive mlKind : Type :=
+  MSort
+| MVar (s: mlSort)
+| MCst (s: mlSort)
+| MRel (al: list mlSort)
+| MError.
+
+Definition isMLSort k := match k with MSort => True | _ => False end.
+Definition isMLRel k := match k with MRel _ => True | _ => False end.
+Definition isMLVar k := match k with MVar _ => True | _ => False end.
+Definition isMLCst k := match k with MCst _ => True | _ => False end.
+
+Definition isMLSortDec k : {isMLSort k}+{not(isMLSort k)} :=
+  match k return {isMLSort k}+{not(isMLSort k)} with MSort => left I | _ => right (fun h => match h:False with end) end.
+
+Definition isMLVarDec k : {isMLVar k}+{not(isMLVar k)} :=
+  match k return {isMLVar k}+{not(isMLVar k)} with MVar _ => left I | _ => right (fun h => match h:False with end) end.
+
+Definition isMLCstDec k : {isMLCst k}+{not(isMLCst k)} :=
+  match k return {isMLCst k}+{not(isMLCst k)} with MCst _ => left I | _ => right (fun h => match h:False with end) end.
+
+Definition isMLRelDec k : {isMLRel k}+{not(isMLRel k)} :=
+  match k return {isMLRel k}+{not(isMLRel k)} with MRel _ => left I | _ => right (fun h => match h:False with end) end.
 
 Record mlSig := {
-  mlSorts : list mlSort;
-  mlRelations : list mlRelation;
-  mlConstants: list mlConstant;
+  mlIdents : list string;
+  mlKinds : string -> mlKind;
   mlClosures: list mlPath;
+(* auxiliairy *)
+  isMLSortB s := if isMLSortDec (mlKinds s) then true else false;
+  isMLVarB s := if isMLVarDec (mlKinds s) then true else false;
+  isMLCstB s := if isMLCstDec (mlKinds s) then true else false;
+(* WF *)
+  mlSorts: list mlSort := List.filter isMLSortB mlIdents;
+  mlVwf: forall v s, mlKinds v = MVar s -> List.In s mlSorts;
+  mlCwf: forall v s, mlKinds v = MCst s -> List.In s mlSorts;
+  mlRwf: forall v sl, mlKinds v = MRel sl -> forall s, List.In s sl -> List.In s mlSorts;
 }.
 
+Module Type MLSignature.
+  Parameter sg: mlSig.
+End MLSignature.
+
+Module MLCervino(Sg: MLSignature).
+
+Record mlVariable := {
+  mlVarName: string;
+  mlVar_dcl : isMLVar (mlKinds Sg.sg mlVarName);
+  mlVar_in : List.In mlVarName (mlIdents Sg.sg)
+}.
+
+Definition mlVarSort (r: mlVariable): mlSort :=
+  match mlKinds Sg.sg (mlVarName r) as k return isMLVar k -> _ with
+    MVar s => fun h => s
+  | _ => fun h => match h with end
+  end (mlVar_dcl r).
+
+Lemma mlVariableWF: forall v, mlKinds Sg.sg (mlVarName v) = MVar (mlVarSort v).
+Proof.
+  intros.
+  destruct v as [n d].
+  unfold mlVarSort; simpl.
+  destruct (mlKinds Sg.sg n); simpl in *; tauto.
+Qed.
+
+Definition mlAllVariables :=
+  imap_filter (fun id => isMLVarDec (mlKinds Sg.sg id))
+    (mlIdents Sg.sg)
+    (fun v h1 h2 => {| mlVarName := v; mlVar_dcl := h1; mlVar_in := h2 |}).
+
+Definition mlVariables s :=
+  List.filter (fun v => if string_dec (mlVarSort v) s then true else false) mlAllVariables.
+
+Record mlConstant := {
+  mlCstName: string;
+  mlCst_dcl : isMLCst (mlKinds Sg.sg mlCstName);
+  mlCst_in : List.In mlCstName (mlIdents Sg.sg)
+}.
+
+Definition mlCstSort (r: mlConstant): mlSort :=
+  match mlKinds Sg.sg (mlCstName r) as k return isMLCst k -> _ with
+    MCst s => fun h => s
+  | _ => fun h => match h with end
+  end (mlCst_dcl r).
+
+Lemma mlConstantWF: forall v, mlKinds Sg.sg (mlCstName v) = MCst (mlCstSort v).
+Proof.
+  intros.
+  destruct v as [n d].
+  unfold mlCstSort; simpl.
+  destruct (mlKinds Sg.sg n); simpl in *; tauto.
+Qed.
+
+Definition mlAllConstants :=
+  imap_filter (fun id => isMLCstDec (mlKinds Sg.sg id))
+    (mlIdents Sg.sg)
+    (fun v h1 h2 => {| mlCstName := v; mlCst_dcl := h1; mlCst_in := h2 |}).
+
+Definition mlConstants s :=
+  List.filter (fun v => if string_dec (mlCstSort v) s then true else false) mlAllConstants.
+
+Record mlRelation := {
+  mlRelName: string;
+  mlRel_dcl : isMLRel (mlKinds Sg.sg mlRelName);
+  mlRel_in : List.In mlRelName (mlIdents Sg.sg);
+}.
+
+Definition mlRelArity (r: mlRelation) :=
+  match mlKinds Sg.sg (mlRelName r) as k return isMLRel k -> _ with
+    MRel al => fun h => al
+  | _ => fun h => match h with end
+  end (mlRel_dcl r).
+
+Lemma mlRelationWF: forall r, mlKinds Sg.sg (mlRelName r) = MRel (mlRelArity r).
+Proof.
+  intros.
+  destruct r as [n d]; simpl.
+  unfold mlRelArity; simpl.
+  destruct (mlKinds Sg.sg n); simpl in *; tauto.
+Qed.
+
+Definition mlRelations :=
+  imap_filter (fun id => isMLRelDec (mlKinds Sg.sg id))
+    (mlIdents Sg.sg)
+    (fun v h1 h2 => {| mlRelName := v; mlRel_dcl := h1; mlRel_in := h2 |}).
+
 Inductive mlTerm : Type :=
-  MLVar: mlVar -> mlTerm
-| MLCst: mlConstant -> mlTerm.
+  MLVar (v: mlVariable)
+| MLCst (c: mlConstant).
+
+Definition mlTermSort (tm: mlTerm): mlSort :=
+  match tm with
+    MLVar v => mlVarSort v
+  | MLCst c => mlCstSort c
+  end.
+
+Lemma mlTwf: forall t, List.In (mlTermSort t) (mlSorts Sg.sg).
+Proof.
+  intros.
+  destruct t; simpl.
+  apply mlVwf with (v:=mlVarName v); simpl.
+  generalize (mlVar_dcl v); intro.
+  destruct v as [n d]; simpl in *.
+  unfold mlVarSort; simpl.
+  destruct (mlKinds Sg.sg n); simpl in *; tauto.
+
+  apply mlCwf with (v:=mlCstName c); simpl.
+  generalize (mlCst_dcl c); intro.
+  destruct c as [n d]; simpl in *.
+  unfold mlCstSort; simpl.
+  destruct (mlKinds Sg.sg n); simpl in *; tauto.
+Qed.
+
+Definition isMLLit (r: mlRelation) (args: list mlTerm): Prop := 
+  mlRelArity r = List.map mlTermSort args.
 
 Inductive mlLiteral: Type :=
-  MLPApp: nat -> mlRelation -> list mlTerm -> mlLiteral.
+  MLPApp (nx: nat) (r: mlRelation) (args: list mlTerm) (wf: isMLLit r args).
 
 Inductive mlAtom: Type :=
-| MLLiteral: mlLiteral -> mlAtom
-| MLNLiteral: mlLiteral -> mlAtom
-| MLEq: mlSort -> mlTerm -> mlTerm -> mlAtom
-| MLNEq: mlSort -> mlTerm -> mlTerm -> mlAtom.
+| MLLiteral (lt: mlLiteral)
+| MLNLiteral (lt: mlLiteral)
+| MLEq (s: mlSort) (t1: mlTerm) (t2: mlTerm) (hs1: mlTermSort t1 = s) (hs2: mlTermSort t2 = s)
+| MLNEq (s: mlSort) (t1: mlTerm) (t2: mlTerm) (hs1: mlTermSort t1 = s) (hs2: mlTermSort t2 = s).
 
 Inductive mlFormula: Type :=
-  FTrue: mlFormula
-| FFalse: mlFormula
-| Atom: mlAtom -> mlFormula
-| And: mlFormula -> mlFormula -> mlFormula 
-| Or: mlFormula -> mlFormula -> mlFormula
-| Ex: mlVar -> mlFormula -> mlFormula
-| All: mlVar -> mlFormula -> mlFormula
-| F: mlFormula -> mlFormula
-| G: mlFormula -> mlFormula.
+  MLFTrue: mlFormula
+| MLFFalse: mlFormula
+| MLAtom: mlAtom -> mlFormula
+| MLAnd: mlFormula -> mlFormula -> mlFormula 
+| MLOr: mlFormula -> mlFormula -> mlFormula
+| MLEx: mlVariable -> mlFormula -> mlFormula
+| MLAll: mlVariable -> mlFormula -> mlFormula
+| MLF: mlFormula -> mlFormula
+| MLG: mlFormula -> mlFormula.
 
 Definition mlEvMod := list mlTerm.
 
@@ -65,14 +197,14 @@ Record mlEvModify := {
 
 Record mlEvent := {
   mlEvName : string;
-  mlEvArgs : list mlVar;
+  mlEvArgs : list mlVariable;
   mlEvBody : mlFormula;
   mlEvModifies : list mlEvModify;
 }.
 
 Inductive mlUsing :=
   TEA: mlUsing (* transfo Ex -> Alll avec intro E *)
-| TTC: mlRelation -> mlVar -> mlFormula -> mlUsing (* transitive closure *)
+| TTC: mlRelation -> mlVariable -> mlFormula -> mlUsing (* transitive closure *)
 | TFC: (mlEvent -> mlFormula) -> mlUsing. (* frame condition *)
 
 Record mlCheck := {
@@ -83,17 +215,19 @@ Record mlCheck := {
 }.
 
 Record mlModel := {
-  mlMySig : mlSig;
   mlAxioms: list mlFormula;
   mlEvents: list mlEvent;
 }.
 
-Record mlSignedFormula := {
-  mlSfSig : mlSig;
+(***
+Record mlSignedFormula := { (* A REVOIR: changement de signature *)
   mlSfForm : mlFormula;
 }.
 
-Definition mlTransform (m: mlModel) (chk: mlCheck) : option mlSignedFormula := None.
+Definition mlTransform (m: mlModel) (chk: mlCheck) : option mlSignedFormula.
+Admitted.
+***)
+End MLCervino.
 
 Require Extraction.
 
@@ -101,8 +235,9 @@ Require Import Coq.extraction.ExtrOcamlBasic.
 
 Require Import extraction.ExtrOcamlString.
 Extract Inlined Constant String.append => "(^)".
+Extract Inlined Constant String.string_dec => "(=)".
 Extract Inductive string => "string" [ """""" "(fun (a, b) -> (String.make 1 a) ^ b)"] "(fun e c s -> if s = """" then e else c s.[0] (String.sub s 1 (String.length s - 1)))".
 
-Extract Inductive nat => int [ "0" "succ" ] "(fun fO fS n -> if n = 0 then fO () else fS (n - 1))".
+Extract Inductive nat => int [ "0" "succ" ] "(fun fO fS n -> if n=0 then fO () else fS (n-1))".
 
-Extraction "api.ml" mlTransform.
+Extraction "/tmp/generate.ml" MLCervino.
