coq/api2coq.v
@@ -1,0 +1,239 @@
+Add LoadPath "$HOME/COQ/FO-LTL" as Top.
+
+Require Import String.
+Require Import List.
+Require Coq.Arith.PeanoNat.
+Require Import ProofIrrelevance.
+Require Import Init.Logic.
+Import  EqNotations.
+
+Require Import Top.api.
+Require Import Top.foltl.
+Require Import Top.finite.
+Require Import Top.dec.
+Require Import Top.utils.
+
+Instance StrDec : EqDec := {| eq_dec := string_dec |}.
+Instance NatDec : EqDec := {| eq_dec := Coq.Arith.PeanoNat.Nat.eq_dec |}.
+
+Module ML2Coq (Sg: MLSignature).
+Module Import Cervino := MLCervino(Sg).
+
+Definition mlSorts2Sort : SortT := asFinite (mlSorts Sg.sg).
+Definition mlSort2Sort (s: mlSort) (h: List.In s (mlSorts Sg.sg)) : mlSorts2Sort :=
+ exist _ s h.
+
+Instance mlVariableDec: @EqDec mlVariable.
+Proof.
+  split; repeat intro.
+  destruct x as [v1 h1]; destruct y as [v2 h2].
+  destruct (string_dec v1 v2); [left|right].
+  subst v2.
+  f_equal.
+  apply proof_irrelevance.
+  apply proof_irrelevance.
+
+  intro.
+  injection H; clear H; intro.
+  apply (n H).
+Defined.
+
+Instance mlConstantDec: @EqDec mlConstant.
+Proof.
+  split; repeat intro.
+  destruct x as [v1 h1]; destruct y as [v2 h2].
+  destruct (string_dec v1 v2); [left|right].
+  subst v2.
+  f_equal.
+  apply proof_irrelevance.
+  apply proof_irrelevance.
+  intro.
+  injection H; clear H; intro.
+  apply (n H).
+Defined.
+
+Instance mlRelationDec: @EqDec mlRelation.
+Proof.
+  split; repeat intro.
+  destruct x as [v1 h1]; destruct y as [v2 h2].
+  destruct (string_dec v1 v2); [left|right].
+  subst v2.
+  f_equal.
+  apply proof_irrelevance.
+  apply proof_irrelevance.
+  intro.
+  injection H; clear H; intro.
+  apply (n H).
+Defined.
+
+(*
+Definition mlRelDec : EqDec (T := mlRelation).
+Proof.
+  split; repeat intro.
+  destruct x as [n1 a1 l1]; destruct y as [n2 a2 l2].
+  destruct (string_dec n1 n2).
+  subst n2; left.
+Defined.
+
+Definition mlRels2Rels : EqDec (T:=StrDec) :=
+  (List.map mlRelName (mlConstants srcSig))).
+*)
+
+Definition coqSig : Sig := {|
+  Sort := mlSorts2Sort;
+  variable s := asFinite (mlVariables (proj1_sig s));
+  constant s := asFinite (mlConstants (proj1_sig s));
+  predicate := asFinite mlRelations;
+  pr_arity p := List.length (mlRelArity (proj1_sig p));
+  pr_args p i := 
+    mlSort2Sort (fnth (mlRelArity (proj1_sig p)) i)
+                  (mlRwf Sg.sg (mlRelName (proj1_sig p)) 
+                                  _
+                                  (mlRelationWF _)
+                                  (fnth (mlRelArity (proj1_sig p)) i)
+                                  (fnth_In _ i))
+|}.
+
+Definition mlSortOfVar v: Sort (Sig:=coqSig) :=
+  (mlSort2Sort (mlVarSort v)
+    (mlVwf Sg.sg (mlVarName v) (mlVarSort v) (mlVariableWF _) )).
+
+Definition mlSortOfCst v: Sort (Sig:=coqSig) :=
+  (mlSort2Sort (mlCstSort v)
+    (mlCwf Sg.sg (mlCstName v) (mlCstSort v) (mlConstantWF _) )).
+
+Definition mlSortOfTerm t: Sort (Sig:=coqSig) := 
+  match t with
+    MLVar v => mlSortOfVar v
+  | MLCst c => mlSortOfCst c
+  end.
+
+Lemma mlSortOfTerm_mlSort2Sort: forall t i,
+  mlSortOfTerm t = mlSort2Sort (mlTermSort t) i.
+Proof.
+  intros.
+  destruct t; simpl.
+  destruct v as [v h1 h2].
+  unfold mlTermSort, mlSortOfVar, mlSort2Sort in *; simpl in *.
+  f_equal.
+  apply proof_irrelevance.
+
+  destruct c as [c h1 h2].
+  unfold mlTermSort, mlSortOfCst, mlSort2Sort in *; simpl in *.
+  f_equal.
+  apply proof_irrelevance.
+Qed.
+
+Program Definition mlVar2Var (v: mlVariable): variable (Sig:=coqSig) (mlSortOfVar v) :=
+  exist _ v _.
+Next Obligation.
+  unfold mlVariables.
+  apply filter_In.
+  split.
+  unfold mlAllVariables.
+  set (f v h1 h2 := {| mlVarName := v; mlVar_dcl := h1; mlVar_in := h2 |}).
+  assert (v = f (mlVarName v) (mlVar_dcl v) (mlVar_in v)). 
+  destruct v; simpl; reflexivity.
+  rewrite H.
+  apply imap_filter_In_intro.
+  destruct (string_dec (mlVarSort v) (mlVarSort v)); tauto.
+Qed.
+
+Program Definition mlCst2Cst (c: mlConstant): constant (Sig:=coqSig) (mlSortOfCst c) :=
+  exist _ c _.
+Next Obligation.
+  unfold mlConstants.
+  apply filter_In.
+  split.
+  unfold mlAllConstants.
+  set (f v h1 h2 := {| mlCstName := v; mlCst_dcl := h1; mlCst_in := h2 |}).
+  assert (c = f (mlCstName c) (mlCst_dcl c) (mlCst_in c)). 
+  destruct c; simpl; reflexivity.
+  rewrite H.
+  apply imap_filter_In_intro.
+  destruct (string_dec (mlCstSort c) (mlCstSort c)); tauto.
+Qed.
+
+Definition mlTerm2Term t : term coqSig (mlSortOfTerm t) :=
+  match t return term coqSig (mlSortOfTerm t) with
+    MLVar v => Var coqSig _ (mlVar2Var v)
+  | MLCst c => Cst coqSig _ (mlCst2Cst c)
+  end.
+
+Program Definition mlRelation2Pred p : predicate (Sig:=coqSig) :=
+  exist _ p _.
+Next Obligation.
+  unfold mlRelations.
+  set (f v h1 h2 := {| mlRelName := v; mlRel_dcl := h1; mlRel_in := h2 |}).
+  assert (p = f (mlRelName p) (mlRel_dcl p) (mlRel_in p)). 
+  destruct p; simpl; reflexivity.
+  rewrite H.
+  apply imap_filter_In_intro.
+Qed.
+
+Program Definition mlLiteral2Literal l : literal coqSig :=
+  match l with
+    MLPApp x p al h => PApp coqSig x (mlRelation2Pred p) 
+      (fun i => mlTerm2Term (fnth al i))
+  end.
+Next Obligation.
+  rewrite h.
+  apply map_length.
+Qed.
+Next Obligation.
+  generalize ((mlRwf Sg.sg (mlRelName p) (mlRelArity p) (mlRelationWF p)
+     (fnth (mlRelArity p) i) (fnth_In (mlRelArity p) i))); intro.
+  generalize (mlLiteral2Literal_obligation_1 p al h); intro.
+  unfold mlRelation2Pred in e; simpl in e.
+  unfold isMLLit in h.
+  revert i i0 e; rewrite h; intros; clear h p x.
+  revert i0; rewrite (fnth_map mlTermSort al i); intro.
+  revert i i0; generalize (map_length mlTermSort al); rewrite e; simpl; intros.
+  rewrite <-mlSortOfTerm_mlSort2Sort.
+  rewrite (proof_irrelevance _ e0 eq_refl); simpl; auto.
+Qed.
+
+Program Definition mlAtom2Atom a : atom coqSig :=
+  match a with
+  | MLLiteral l => Literal coqSig (mlLiteral2Literal l)
+  | MLNLiteral l => NLiteral coqSig (mlLiteral2Literal l)
+  | MLEq s t1 t2 h1 h2 => Eq coqSig (mlSort2Sort s _) (mlTerm2Term t1) (mlTerm2Term t2)
+  | MLNEq s t1 t2 h1 h2 => NEq coqSig (mlSort2Sort s _)  (mlTerm2Term t1) (mlTerm2Term t2)
+  end.
+Next Obligation.
+  apply mlTwf.
+Defined.
+Next Obligation.
+  apply mlSortOfTerm_mlSort2Sort.
+Defined.
+Next Obligation.
+  generalize (mlAtom2Atom_obligation_1 (mlTermSort t1) t1 t2 eq_refl h2).
+  rewrite <-h2.
+  apply mlSortOfTerm_mlSort2Sort.
+Defined.
+Next Obligation.
+  apply mlTwf.
+Defined.
+Next Obligation.
+  apply mlSortOfTerm_mlSort2Sort.
+Defined.
+Next Obligation.
+  generalize (mlAtom2Atom_obligation_4 (mlTermSort t1) t1 t2 eq_refl h2).
+  rewrite <-h2.
+  apply mlSortOfTerm_mlSort2Sort.
+Defined.
+
+Fixpoint mlFormula2formula f: formula coqSig := 
+  match f with
+    MLFTrue => FTrue coqSig
+  | MLFFalse => FFalse coqSig
+  | MLAtom a => Atom coqSig (mlAtom2Atom a)
+  | MLAnd f1 f2 => And coqSig (mlFormula2formula f1) (mlFormula2formula f2)
+  | MLOr f1 f2 => Or coqSig (mlFormula2formula f1) (mlFormula2formula f2)
+  | MLEx v b => Ex coqSig _ (mlVar2Var v) (mlFormula2formula b)
+  | MLAll v b => Ex coqSig _ (mlVar2Var v) (mlFormula2formula b)
+  | MLF f' => F coqSig (mlFormula2formula f')
+  | MLG f' => G coqSig (mlFormula2formula f')
+  end.
+
+End ML2Coq.
