coq/utils.v
@@ -1,0 +1,84 @@
+Add LoadPath "$HOME/COQ/FO-LTL" as Top.
+
+Require Import ProofIrrelevance.
+
+Require Import List.
+Require Import Fin.
+Require Import Init.Logic.
+Import  EqNotations.
+
+Fixpoint imap_filter {T U} {p: T->Prop} (P: forall x, {p x}+{not (p x)}) (l: list T):  (forall x, p x -> List.In x l -> U) -> list U :=
+  match l return (forall x, p x -> List.In x l -> U) -> list U with
+    nil => fun f => nil
+  | cons x l' => match P x with 
+    left hp => fun f => f x hp (or_introl eq_refl)::imap_filter P l' (fun x h1 h2 => f x h1 (or_intror h2))
+   | right _ => fun f => imap_filter P l' (fun x h1 h2 => f x h1 (or_intror h2))
+   end
+  end.
+
+Lemma imap_filter_In_intro: forall T U {p: T->Prop} (P: forall x, {p x}+{not (p x)}) (l: list T) (f: forall x, p x -> List.In x l -> U),
+  forall x (h1: p x) (h2: In x l), List.In (f x h1 h2) (imap_filter P l f).
+Proof.
+  induction l; simpl; intros; auto.
+  destruct (P a); try tauto.
+  destruct h2.
+  subst x.
+  left.
+  f_equal.
+  apply proof_irrelevance.
+  right.
+  apply (IHl (fun x h1 h2 => f x h1 (or_intror h2)) x h1 i).
+  destruct h2.
+  subst x; destruct (n h1).
+  apply (IHl (fun x h1 h2 => f x h1 (or_intror h2)) x h1 i).  
+Qed.
+
+Fixpoint map_filter {T U} {p: T->Prop} (P: forall x, {p x}+{not (p x)}) (f: forall x, p x -> U) (l: list T): list U :=
+  match l with
+    nil => nil
+  | cons x l' => match P x with 
+    left h => f x h::map_filter P f l'
+   | right _ => map_filter P f l'
+   end
+  end.
+
+Fixpoint fnth {T} (l: list T):  Fin.t (List.length l) -> T :=
+  match l as l return Fin.t (List.length l) -> T with
+    nil => case0 _
+  | cons x l' => fun (i: Fin.t (S (List.length l'))) =>
+    caseS' i (fun _ => T) x (fun j => fnth l' j)
+  end.
+
+Lemma fnth_In: forall {T} (l: list T) (i: Fin.t (List.length l)),
+  List.In (fnth l i) l.
+Proof.
+  induction l; simpl; intros; auto.
+  inversion i.
+  apply (caseS' i); simpl; intros; auto.
+Qed.
+
+Lemma fnth_map: forall {T U} (f: T->U) (l: list T) (i: Fin.t (List.length (List.map f l))),
+  fnth (map f l) i = f (fnth l (rew (map_length f l) in i)).
+Proof.
+  induction l; simpl; intros; auto.
+  inversion i.
+  
+  apply (caseS' i); simpl; intros; auto.
+  f_equal.
+  generalize (map_length f (a::l)); simpl; intro.
+  generalize (fun j : t (length l) => fnth l j) as g.
+  injection e; intro e'.
+  revert i e; rewrite <-e'; intros.
+  rewrite (proof_irrelevance _ e eq_refl); simpl; now auto.
+  
+  rewrite IHl; clear IHl.
+  f_equal.
+  generalize (map_length f (a::l)); simpl; intro.
+  injection e; intro e'.
+  rewrite (proof_irrelevance _ _ e').
+  assert ((rew [t] e in FS p) = FS (rew [t] e' in p)).
+  revert e p; rewrite e'; simpl; intros.
+  rewrite (proof_irrelevance _ e eq_refl); simpl; now auto.
+  rewrite H; simpl; now auto.
+Qed.
+
