coq/varset.v
@@ -1,0 +1,307 @@
+Add LoadPath "$HOME/COQ/FO-LTL" as Top.
+
+Require Import ProofIrrelevance.
+Require Import Eqdep_dec.
+
+Require Import Top.foltl.
+Require Import Top.set.
+Require Import Top.dec.
+Require Import Top.finite.
+
+Section VarSet.
+
+Context {Ts: Type} {Tv: Ts->Type} {Tc: Ts->Type} {Tp: Type}.
+Variable Sg: @Sig Ts Tv Tc Tp.
+
+
+Definition VarSet := forall s, SV.set (variable s).
+
+Definition vsIn {s} (v: variable s) (F: VarSet) := SV.set_In v (F s).
+
+Definition vsSubset e1 e2 := forall s, SV.subset (T:=variable s) (e1 s) (e2 s).
+
+Lemma vsSubset_refl : forall e, vsSubset e e.
+Proof.
+  repeat intro; auto.
+Qed.
+
+Lemma vsSubset_trans : forall {e1 e2 e3}, vsSubset e1 e2 -> vsSubset e2 e3 -> vsSubset e1 e3.
+Proof.
+  repeat intro; auto.
+  apply H0.
+  apply H.
+  auto.
+Qed.
+
+Definition vsAdd {s} (v: variable s) (e: VarSet): VarSet :=
+  fun s' =>
+    match eq_dec s s' with
+      left h => match h in _=s' return SV.set (variable s') with 
+                  eq_refl => SV.add v (e s)
+                end
+    | right _ => e s'
+    end.
+
+Lemma vsAdd_l: forall {s} (v: variable s) (e: VarSet),
+  SV.set_In v (vsAdd v e s).
+Proof.
+  unfold vsAdd; simpl; intros.
+  destruct (eq_dec s s); try tauto.
+  rewrite (proof_irrelevance _ e0 eq_refl).
+  apply SV.InAdd_l.
+Qed.
+
+Lemma vsAdd_r: forall {s s'} (v: variable s) (e: VarSet) {w: variable s'},
+  SV.set_In w (e s') -> SV.set_In w (vsAdd v e s').
+Proof.
+  intros.
+  unfold vsAdd.
+  destruct (eq_dec s s'); auto.
+  subst s'.
+  apply SV.InAdd_r; auto.
+Qed.
+
+Lemma vsAdd_elim: forall {s s'} (v: variable s) (e: VarSet) {w: variable s'},
+  SV.set_In w (vsAdd v e s') -> isEq2 (U:=variable) s' w s v \/ SV.set_In w (e s').
+Proof.
+  intros.
+  unfold vsAdd in H.
+  unfold isEq2; simpl.
+  destruct (eq_dec s s').
+  subst s'.
+  apply SV.InAdd in H; destruct H.
+  subst v.
+  left; auto.
+  right; auto.
+  right; auto.
+Qed.
+
+Lemma vsAdd_ne: forall {s s'} {v: variable s} {e: VarSet} {w: variable s'},
+  SV.set_In w (vsAdd v e s') -> not (isEq2 (U:=variable) s' w s v) -> SV.set_In w (e s').
+Proof.
+  intros.
+  apply vsAdd_elim in H.
+  destruct H; tauto.
+Qed.
+
+Lemma vsAdd_ne2: forall {s s'} {v: variable s} {e: VarSet} {w: variable s'},
+  SV.set_In w (vsAdd v e s') -> not (SV.set_In w (e s')) -> (isEq2 (U:=variable) s' w s v).
+Proof.
+  intros.
+  apply vsAdd_elim in H.
+  destruct H; tauto.
+Qed.
+
+Definition vsEmpty: VarSet := fun s => SV.empty _.
+
+Definition vsSing {s} (v: variable s): VarSet :=
+  fun s' =>
+    match eq_dec s s' with
+      left h => match h in _=s' return SV.set (variable s') with 
+                  eq_refl => SV.sing _  v
+                end
+    | right _ => SV.empty _
+    end.
+
+Definition vsUnion (e1 e2: VarSet): VarSet :=
+  fun s => SV.union (e1 s) (e2 s).
+
+Lemma vsUnion_l: forall {s v} {e1 e2: VarSet},
+  SV.set_In v (e1 s) -> SV.set_In v (vsUnion e1 e2 s).
+Proof.
+  intros.
+  apply SV.InUnion_l; auto.
+Qed.
+
+Lemma vsUnion_r: forall {s v} {e1 e2: VarSet},
+  SV.set_In v (e2 s) -> SV.set_In v (vsUnion e1 e2 s).
+Proof.
+  intros.
+  apply SV.InUnion_r; auto.
+Qed.
+
+Lemma vsUnion_elim: forall {s v} {e1 e2: VarSet},
+  SV.set_In v (vsUnion e1 e2 s) -> SV.set_In v (e1 s) \/ SV.set_In v (e2 s).
+Proof.
+  intros.
+  apply SV.InUnion in H.
+  destruct H; tauto.
+Qed.
+
+Definition vsInter (e1 e2: VarSet): VarSet :=
+  fun s => SV.inter (e1 s) (e2 s).
+
+Lemma vsInter_intro: forall {s v} {e1 e2: VarSet},
+  SV.set_In v (e1 s) -> SV.set_In v (e2 s) -> SV.set_In v (vsInter e1 e2 s).
+Proof.
+  intros.
+  apply SV.InInter; auto.
+Qed.
+
+Lemma vsInter_elim: forall {s v} {e1 e2: VarSet},
+  SV.set_In v (vsInter e1 e2 s) -> SV.set_In v (e1 s) /\ SV.set_In v (e2 s).
+Proof.
+  intros; split.
+  apply SV.InInter_l in H; auto.
+  apply SV.InInter_r in H; auto.
+Qed.
+
+Definition vsGUnion `{K: Finite} (ek: K->VarSet): VarSet :=
+  fun s => SV.GUnion (T1:=K) (T2:=variable s) fin_set fin_set (fun k _ => ek k s).
+
+Lemma vsGUnion_intro `{K:Finite} {ek: K->VarSet}:
+  forall s k, SV.subset (ek k s) (vsGUnion ek s).
+Proof.
+  repeat intro.
+  unfold vsGUnion.
+  apply SV.InCUnion_intro with (u:=k); simpl; auto.
+  apply fin_all.
+  apply fin_all.
+Qed.
+
+Lemma vsGUnion_elim `{K:Finite} {ek: K->VarSet} s (v: variable s):
+  vsIn v (vsGUnion ek) -> exists k, vsIn v (ek k).
+Proof.
+  repeat intro.
+  unfold vsGUnion in H.
+  apply SV.InCUnion_elim in H; simpl; auto.
+  destruct H as [k [h1 [h2 h3]]].
+  exists k.
+  apply h3.
+  apply h2.
+Qed.
+
+Lemma vsSubsetUnion_elim_l: forall e1 e2 e,
+  vsSubset (vsUnion e1 e2) e -> vsSubset e1 e.
+Proof.
+  repeat intro.
+  apply (H s v); clear H; intros.
+  apply vsUnion_l; auto.
+Qed.
+
+Lemma vsSubsetUnion_elim_r: forall e1 e2 e,
+  vsSubset (vsUnion e1 e2) e -> vsSubset e2 e.
+Proof.
+  repeat intro.
+  apply (H s v); clear H; intros.
+  apply vsUnion_r; auto.
+Qed.
+
+Lemma vsSubsetGUnion_elim `{K:Finite} {ek: K->VarSet} e:
+  vsSubset (vsGUnion ek) e -> forall k, vsSubset (ek k) e.
+Proof.
+  repeat intro.
+  unfold vsGUnion.
+  apply (H s v); clear H.
+  apply SV.InCUnion_intro with (u:=k); simpl; auto.
+  apply fin_all.
+  apply fin_all.
+Qed.
+
+Definition vsRemove {s} (v: variable s) (e: VarSet): VarSet :=
+  fun s' => match eq_dec s s' with
+    left h =>
+      match h in _=s' return SV.set (variable s') with
+        eq_refl => SV.remove v (e s)
+      end
+  | right _ => e s'
+  end.
+
+Lemma vsInRemove_intro: forall s (v: variable s) (e: VarSet) s' (w: variable s'),
+  vsIn w e -> not (isEq2 (U:=variable) s v s' w) -> vsIn w (vsRemove v e).
+Proof.
+  intros.
+  unfold vsRemove, vsIn; simpl.
+  destruct (eq_dec s s'); auto.
+  subst s'.
+  apply SV.InRemove.
+  intro.
+  subst w.
+  apply H0; reflexivity.
+  apply H.
+Qed.
+
+Lemma vsInRemove_elim: forall s (v: variable s) (e: VarSet) s' (w: variable s'),
+  vsIn w (vsRemove v e) -> vsIn w e /\ not (isEq2 (U:=variable) s v s' w).
+Proof.
+  intros.
+  unfold vsRemove, vsIn in H.
+  destruct (eq_dec s s'); auto.
+  subst s'.
+  split.
+  apply SV.InRemove_r in H; apply H.
+  apply SV.InRemove_l in H.
+  simpl; intro.
+  apply H; clear H.
+  apply inj_pair2_eq_dec in H0; try apply eq_dec.
+  symmetry; apply H0.
+
+  split.
+  apply H.
+  intro; apply n; clear n.
+  injection H0; intro; auto.  
+Qed.
+
+Definition vsFinite (vs: VarSet): Finite :=
+  PairFin Sort (fun s => asFinite (vs s)).
+
+Lemma vsSing_intro: forall s v, SV.set_In v (vsSing v s).
+Proof.
+  intros.
+  unfold vsSing.
+  destruct (eq_dec s s); try tauto.
+  rewrite (proof_irrelevance _ e eq_refl).
+  left; auto.
+Qed.
+
+Lemma vsSing_elim: forall s (v: variable s) s' (w: variable s'), 
+  SV.set_In v (vsSing w s) -> isEq2 (U:=variable) s v s' w.
+Proof.
+  intros.
+  unfold vsSing in H.
+  unfold isEq2; simpl.
+  destruct (eq_dec s' s); try tauto; subst.
+  destruct H; try tauto; subst; auto.
+Qed.
+
+Lemma vsSubsetSing: forall {s} {v: variable s} e, vsSubset (vsSing v) e -> SV.set_In v (e s).
+Proof.
+  intros.
+  apply SV.subset_sing; repeat intro.
+  generalize (H s v0); intro.
+  apply H1.
+  destruct H0.
+  subst v0.
+  apply vsSing_intro.
+  destruct H0.
+Qed.
+
+Definition vsVars `{K: Finite} {sk: K->Sort} (vk: forall k, variable (sk k)) : VarSet :=
+  vsGUnion (fun k => vsSing (vk k)).
+
+Lemma vsVars_intro: forall `{K: Finite} {sk: K->Sort} (vk: forall k, variable (sk k)),
+  forall k, SV.set_In (vk k) (vsVars vk (sk k)).
+Proof.
+  intros.
+  apply SV.InCUnion_intro with (u:=k); auto.
+  apply fin_all; simpl; intros; auto.
+  apply fin_all.
+  intro.
+  apply vsSing_intro.
+Qed.
+
+Lemma vsVars_elim: forall `{K: Finite} {sk: K->Sort} (vk: forall k, variable (sk k)),
+  forall s (v: variable s), SV.set_In v (vsVars vk s) -> exists k, isEq2 (U:=variable) (sk k) (vk k) s v.
+Proof.
+  intros.
+  unfold vsVars in H.
+  apply SV.InCUnion_elim in H.
+  destruct H as [u [h1 [h2 h3]]].
+  exists u; unfold isEq2; simpl.
+  apply h3 in h2; clear h3.
+  apply vsSing_elim in h2.
+  symmetry; apply h2.
+Qed.
+
+End VarSet.
+
